Support modifies in ModularInterop

vale/code/arch/x64/interop/ModularInterop.fst
@@ -16,11 +16,8 @@ let to_b8 m =
   prove_squash (h_equals_refine b8 m (MS.buffer (MS.TBase MS.TUInt64)) m) h;
   m
 
-let regs_with_stack (regs:registers) (stack_b:b8) : registers =
-    fun r ->
-      if r = Rsp then
-        IA.addrs stack_b
-      else regs r
+let regs_with_stack (regs:registers) (stack_b:b8) (rsp:nat64) : registers =
+  fun r -> if r = Rsp then rsp else regs r
 
 let create_memory (acc:list b8) (h0:HS.mem{mem_roots_p h0 acc}) : M.mem =
   { MS.addrs = IA.addrs;
@@ -29,6 +26,7 @@ let create_memory (acc:list b8) (h0:HS.mem{mem_roots_p h0 acc}) : M.mem =
 
 let create_initial_trusted_state_core
        (acc:list b8)
+       (rsp:nat64)
        (regs:registers)
        (xmms:xmms_t)
        (taint:taint_map)
@@ -37,7 +35,7 @@ let create_initial_trusted_state_core
   : GTot (TS.traceState & MS.mem)
   = let acc = stack::acc in
     let (mem:MS.mem) = create_memory acc h0 in
-    let regs = FunctionalExtensionality.on reg (regs_with_stack regs stack) in
+    let regs = FunctionalExtensionality.on reg (regs_with_stack regs stack rsp) in
     let xmms = FunctionalExtensionality.on xmm xmms in
     let (s0:BS.state) = {
       BS.ok = true;
@@ -55,13 +53,14 @@ let create_initial_trusted_state_core
 
 let create_initial_vale_state_core
        (acc:list b8)
+       (rsp:nat64)
        (regs:registers)
        (xmms:xmms_t)
        (taint:taint_map)
        (h0:HS.mem)
        (stack:b8{mem_roots_p h0 (stack::acc)})
   : GTot V.va_state
-  = let t_state, mem = create_initial_trusted_state_core acc regs xmms taint h0 stack in
+  = let t_state, mem = create_initial_trusted_state_core acc rsp regs xmms taint h0 stack in
     { VS.ok = TS.(BS.(t_state.state.ok));
       VS.regs = X64.Vale.Regs.of_fun TS.(BS.(t_state.state.regs));
       VS.xmms =  X64.Vale.Xmms.of_fun TS.(BS.(t_state.state.xmms));
@@ -145,6 +144,7 @@ let wrap code pre post v = fun (x0:M.buffer64) (x1:M.buffer64) ->
   HST.push_frame();
   let h1 = HST.get () in
   let (stack_b:b8) = LB.alloca (UInt8.uint_to_t 0) (UInt32.uint_to_t 24) in
+  lemma_low_assumptions_length stack_b;
   let h2 = HST.get () in
   assert (HS.fresh_frame h0 h1);
   assert (disjoint_or_eq_l_aux x0 []);
@@ -160,6 +160,7 @@ let wrap code pre post v = fun (x0:M.buffer64) (x1:M.buffer64) ->
     #(x:(V.va_state & V.va_state & V.va_fuel){
       let (va_s0, va_s1, fuel) = x in
       low_assumptions h0 va_s0.VS.mem x0 x1 /\
+      LB.modifies (LB.loc_union (LB.loc_buffer (to_b8 stack_b)) (LB.loc_union (LB.loc_buffer (to_b8 x0)) (LB.loc_buffer (to_b8 x1)))) h2 va_s1.VS.mem.MS.hs /\
       post IA.win x0 x1 va_s0 stack_b va_s1 fuel
     })
     (fun h0' -> h0' == h2) (fun h0' ->
@@ -172,39 +173,34 @@ let wrap code pre post v = fun (x0:M.buffer64) (x1:M.buffer64) ->
       in
     let regs = upd_reg IA.win regs 0 (IA.addrs x0) in
     let regs = upd_reg IA.win regs 1 (IA.addrs x1) in
-    let va_s0 = create_initial_vale_state_core acc regs xmms taints h0' stack_b in
+    let rsp = IA.addrs stack_b + 24 in
+    let va_s0 = create_initial_vale_state_core acc rsp regs xmms taints h0' stack_b in
     assert (LB.frameOf stack_b = HS.get_tip h0');
     assert (LB.live h0' stack_b);
     let va_mem = va_s0.VS.mem in
     let num_stack_slots = 3 in
-    let num_stack_slots' = 0 in
     assert (low_assumptions h0 va_mem x0 x1);
-
     assert_norm (List.memP x0 [stack_b; x0; x1]);
     assert_norm (List.memP x1 [stack_b; x0; x1]);
     assert (M.buffer_readable va_mem x0);
     assert (M.buffer_readable va_mem x1);
-
-    assert (V.valid_stack_slots va_mem (VS.eval_reg Rsp va_s0) stack_b num_stack_slots' va_s0.VS.memTaint);
-
-    lemma_low_assumptions_length stack_b;
+    assert (V.valid_stack_slots va_mem (VS.eval_reg Rsp va_s0) stack_b num_stack_slots va_s0.VS.memTaint);
     assert (M.buffer_length #(M.TBase M.TUInt64) stack_b >= num_stack_slots);
     assert (M.locs_disjoint ([M.loc_buffer #(M.TBase M.TUInt64) stack_b; M.loc_buffer #(M.TBase M.TUInt64) x0; M.loc_buffer #(M.TBase M.TUInt64) x1]));
-
     assert (M.valid_taint_buf64 x0 va_s0.VS.mem va_s0.VS.memTaint Secret);
     assert (M.valid_taint_buf64 x1 va_s0.VS.mem va_s0.VS.memTaint Secret);
-
     assert (pre IA.win x0 x1 va_s0 stack_b);
     let va_s1, fuel = v IA.win x0 x1 va_s0 stack_b in
     assert (post IA.win x0 x1 va_s0 stack_b va_s1 fuel);
+    assert (V.modifies_mem (M.loc_union (M.loc_buffer x0) (M.loc_buffer x1)) va_s0.VS.mem va_s1.VS.mem);
+    assert (LB.modifies (LB.loc_union (LB.loc_buffer (to_b8 stack_b)) (LB.loc_union (LB.loc_buffer (to_b8 x0)) (LB.loc_buffer (to_b8 x1)))) h2 va_s1.VS.mem.MS.hs);
     ((va_s0, va_s1, fuel), va_s1.VS.mem.MS.hs)
   ) in //conveniently, st_put assumes that the shape of the stack did not change
-  //let h3 = HST.get () in
-  //assert (LB.modifies (LB.loc_union (LB.loc_buffer (to_b8 stack_b)) (LB.loc_union (LB.loc_buffer (to_b8 x0)) (LB.loc_buffer (to_b8 x1)))) h0 h3);
-  //assert (post IA.win x0 x1 va_s0 stack_b va_s1);
+  let h3 = HST.get () in
+  assert (LB.modifies (LB.loc_union (LB.loc_buffer (to_b8 stack_b)) (LB.loc_union (LB.loc_buffer (to_b8 x0)) (LB.loc_buffer (to_b8 x1)))) h2 h3);
   HST.pop_frame ();
   let h4 = HST.get () in
-  //TODO: assert (LB.modifies (LB.loc_union (LB.loc_buffer (to_b8 x0)) (LB.loc_buffer (to_b8 x1))) h0 h4);
+  assert (LB.modifies (LB.loc_union (LB.loc_buffer (to_b8 x0)) (LB.loc_buffer (to_b8 x1))) h0 h4);
   assert (low_assumptions h0 va_s0.VS.mem x0 x1);
   assert (low_assumptions h4 va_s1.VS.mem x0 x1);
   assert (post IA.win x0 x1 va_s0 stack_b va_s1 fuel);
